\documentclass[12pt]{article}
\setlength{\oddsidemargin}{0in}
\setlength{\evensidemargin}{0in}
\setlength{\textwidth}{6.5in}
\setlength{\parindent}{0in}
\setlength{\parskip}{\baselineskip}

\usepackage{amsmath,amsfonts,amssymb}
\usepackage{amsthm}
\usepackage{subfiles}



\theoremstyle{remark}
\newtheorem{remark}{Remark}
\title{Solution to 2.3 Problem 29}

\begin{document}
\maketitle

Question: Find $$ \lim_{t \rightarrow 0} (\frac{1}{t\sqrt{1+t}} - \frac{1}{t}) $$

Solution: $$ \lim_{t \rightarrow 0} (\frac{1}{t\sqrt{1+t}} - \frac{1}{t}) = 
\lim_{t \rightarrow 0} (\frac{1 - \sqrt{1+t}}{t\sqrt{1+t}}) 
$$
Perform a change of variables using $a = \sqrt{1+t}$. Then $$ a^2 - 1 = t $$

Thus, 
$$\lim_{t \rightarrow 0} (\frac{1 - \sqrt{1+t}}{t\sqrt{1+t}}) = \lim_{a \rightarrow 1} (\frac{1 - a}{a(a^2-1)})  = \lim_{a \rightarrow 1} -(\frac{a - 1}{a(a^2-1)}) = 
\lim_{a \rightarrow 1} -(\frac{1}{a(a+1)}) = -\frac{1}{2}$$ as desired.

\end{document}
